Updated proof structure after discussion with Stefan
Updated proof structure after discussion with Stefan. Stefan has also rewrote the algorithm

Monad_Play Around/DNFP/Dutch_National_Flag_Monad.thy
@@ -48,28 +48,20 @@ lemma distinct_swap[simp]:
 
 value\<open>swap [a,b,c,d,e] 0 4 = [e,b,c,d,a]\<close>
 
-definition init_loop where
-"init_loop \<equiv> do{
-                  h \<leftarrow> get high;
-                  j \<leftarrow> get i;
-                  return (h, j)
-                }"
-
+text\<open>Get i and get low seems not to be necessary\<close>
 definition inc_lowbound where
 "inc_lowbound \<equiv> do{
-                  l \<leftarrow> get low;  
-                  s \<leftarrow> get xs;  
-                  j \<leftarrow> get i;                                   
+                  (l, s, j) \<leftarrow> get (\<lambda>e. (low e, xs e, i e));  
                   put xs_Env (swap s j l);
+                  j \<leftarrow> get i;                                   
                   put i_Env (Suc j);
+                  l \<leftarrow> get low;  
                   put low_Env (Suc l)
                 }"
 
 definition add_high where
 "add_high \<equiv> do{
-                s \<leftarrow> get xs;
-                j \<leftarrow> get i;
-                h \<leftarrow> get high;
+                (s, j, h) \<leftarrow> get (\<lambda>e. (xs e, i e, high e));
                 put xs_Env (swap s j h)
               }"
 
@@ -77,7 +69,8 @@ definition dec_highbound where
 "dec_highbound \<equiv> do{
                     h \<leftarrow> get high;
                     put high_Env (h - 1);
-                    add_high
+                    (s, j, h) \<leftarrow> get (\<lambda>e. (xs e, i e, high e));
+                    put xs_Env (swap s j h)
                 }"
 
 definition inc_index where
@@ -88,19 +81,18 @@ definition inc_index where
 
 definition loop_update_action where
 "loop_update_action \<equiv> 
-do{
-  s \<leftarrow> get xs;
-  j \<leftarrow> get i;
-  (if s!j < 1 then do {
-    inc_lowbound
-  }else (if s!j = 2 then do 
-  {
-    dec_highbound
-  }
- else do {
-    inc_index
- }))
-}"
+  do{
+    (s, j) \<leftarrow> get (\<lambda>e. (xs e, i e));
+    (if s!j < 1 then do {
+      inc_lowbound
+    } else (if s!j = 2 then do 
+    {
+      dec_highbound
+    }
+   else do {
+      inc_index
+   }))
+  }"
 
 
 
@@ -109,14 +101,14 @@ fun dnfp_mon:: "nat \<Rightarrow> (env, unit) state" where
 "dnfp_mon 0  = skip"|
 "dnfp_mon (Suc 0)  = skip"|
 "dnfp_mon (Suc n)  = do {
-                        h \<leftarrow> get high;
-                        j \<leftarrow> get i;
+                        (h, j) \<leftarrow> get (\<lambda>e. (high e, i e));
                         (if h > j then do{
                           loop_update_action;
                           dnfp_mon n
                          }
                        else skip
                       )}"
+
 
 definition init_env:: "nat array \<Rightarrow> env" where
   "init_env l \<equiv> \<lparr>high = (length l),            low = 0,
@@ -176,14 +168,15 @@ subsubsection\<open>Pre-conditions\<close>
 definition dnfp_pre where
 "dnfp_pre e \<equiv> high e \<ge> i e
               \<and> i e \<ge> low e 
-              \<and> length (xs e) \<ge> high e"
+              \<and> length (xs e) \<ge> high e
+              \<and> set (xs e) \<subseteq> {1,2,3}"
 
 definition loop_update_action_pre:: "env \<Rightarrow> bool" where
-"loop_update_action_pre e \<equiv>  high e > i e
-                              \<and> length (xs e) > (Suc 0)
-                              \<and> length (xs e) \<ge> high e
-                              \<and> low e < high e
-                              \<and> low e \<le> i e"
+"loop_update_action_pre e \<equiv> high e > i e
+                             \<and> length (xs e) > (Suc 0)
+                             \<and> length (xs e) \<ge> high e
+                             \<and> low e < high e
+                             \<and> low e \<le> i e"
 
 definition loop_update_action_pre_aux:: "env \<Rightarrow> env \<Rightarrow> bool" where
 "loop_update_action_pre_aux e s \<equiv> s = e
@@ -293,6 +286,7 @@ definition inc_index_post:: "env \<Rightarrow> env \<Rightarrow> bool" where
                       \<and> Suc(i e) = i e'
                       \<and> loop_update_action_post e e'"
 
+text\<open>Is it after one iteration of after completion?\<close>
 definition dnfp_post where 
 "dnfp_post e e2 \<equiv> length (xs e) = length (xs e2)
                   \<and> length (xs e) > (Suc 0) \<longrightarrow> (inc_index_post e e2  \<or> dec_highbound_post e e2 \<or> inc_lowbound_post e e2)"
@@ -301,39 +295,195 @@ section\<open>Lemmas\<close>
 subsection\<open>Hoare proofs\<close>
 
 lemma inc_lowbound_spec: "spec (inc_lowbound_pre e) inc_lowbound (GG (inc_lowbound_post e))"
+  unfolding inc_lowbound_pre_def loop_update_action_pre_def GG_def inc_lowbound_post_def loop_update_action_post_def
   apply(simp_all add: inc_lowbound_def)
-  apply(simp add: inc_lowbound_pre_def loop_update_action_pre_def get_def get_state_def)
-  apply (simp_all add: spec_def  get_def get_state_def return_def put_def put_state_def GG_def)
-  apply(simp_all add: inc_lowbound_pre_def loop_update_action_pre_def inc_lowbound_post_def loop_update_action_post_def swap_def xs_Env_def i_Env_def low_Env_def)
-  by linarith
+  apply(intro get_rule; intro allI; simp)
+  apply(intro conj_rule_right)
+         apply(intro seq_rule[of _ _ "(\<lambda>_ y. high e = high y)"])
+          apply (simp add: spec_def put_def put_state_def swap_def get_state_def xs_Env_def i_Env_def)
+  apply(intro allI; simp)
+         apply(intro get_rule; intro allI)
+         apply (intro seq_rule[of _ _ "(\<lambda>_ y. high e = high y)"])
+          apply (simp add: spec_def put_def put_state_def swap_def get_state_def i_Env_def)
+          apply (simp add: spec_def put_def get_def return_def put_state_def swap_def get_state_def low_Env_def)
+  apply (intro seq_rule[of _ _ "(\<lambda>_ y. low e = low y)"])
+          apply (simp add: spec_def put_def put_state_def swap_def get_state_def xs_Env_def i_Env_def)
+        apply(intro allI; simp)
+        apply(intro get_rule; intro allI)
+        apply(intro seq_rule[of _ _ "(\<lambda>_ y. low e = low y)"])
+          apply (simp add: spec_def put_def put_state_def swap_def get_state_def i_Env_def)
+        apply(intro allI; simp)
+        apply(intro get_rule; intro allI)
+        apply(simp add: spec_def put_def get_state_def put_state_def low_Env_def)
+       apply (intro seq_rule[of _ _ "(\<lambda>_ y. length (xs e) = length (xs y))"])
+        apply (simp add: spec_def put_def put_state_def swap_def get_state_def xs_Env_def i_Env_def)
+       apply(intro allI)
+  apply(intro get_rule; intro allI; simp)
+       apply (intro seq_rule[of _ _ "(\<lambda>_ y. length (xs e) = length (xs y))"])
+        apply (simp add: spec_def put_def put_state_def swap_def get_state_def i_Env_def)
+       apply(intro allI; simp)
+       apply(intro get_rule; intro allI)
+       apply(simp add: spec_def put_def get_state_def put_state_def low_Env_def)
+      apply (intro seq_rule[of _ _ "(\<lambda>_ y. high y = high e)"])
+       apply (simp add: spec_def put_def put_state_def swap_def get_state_def xs_Env_def i_Env_def)
+       apply(intro allI; simp)
+       apply(intro get_rule; intro allI)
+  apply (intro seq_rule[of _ _ "(\<lambda>_ y. high y = high e)"])
+       apply (simp add: spec_def put_def put_state_def swap_def get_state_def i_Env_def)
+      apply(intro allI; simp)
+      apply(intro get_rule; intro allI)
+      apply(simp add: spec_def put_def get_state_def put_state_def low_Env_def)
+     apply (intro seq_rule[of _ _ "(\<lambda>_ y. low y = low e)"])
+      apply (simp add: spec_def put_def put_state_def swap_def get_state_def xs_Env_def i_Env_def)
+     apply(intro allI; simp)
+     apply(intro get_rule; intro allI)
+     apply (intro seq_rule[of _ _ "(\<lambda>_ y. low y = low e)"])
+      apply (simp add: spec_def put_def put_state_def swap_def get_state_def i_Env_def)
+     apply(intro allI; simp)
+     apply(intro get_rule; intro allI)
+     apply(simp add: spec_def put_def get_state_def put_state_def low_Env_def)
+     apply (intro seq_rule[of _ _ "(\<lambda>_ y. i y = i e)"])
+     apply (simp add: spec_def put_def put_state_def swap_def get_state_def xs_Env_def i_Env_def)
+    apply(intro allI; simp)
+    apply(intro get_rule; intro allI)
+     apply (intro seq_rule[of _ _ "(\<lambda>_ y. i y > i e)"])
+     apply (simp add: spec_def put_def put_state_def swap_def get_state_def i_Env_def)
+    apply(intro allI; simp)
+    apply(intro get_rule; intro allI)
+    apply(simp add: spec_def put_def get_state_def put_state_def low_Env_def)
+   apply (intro seq_rule[of _ _ "(\<lambda>_ y. i y < high y \<and> i y = i e \<and> high y = high e)"])
+    apply (simp add: spec_def put_def put_state_def swap_def get_state_def xs_Env_def i_Env_def)
+   apply(intro allI; simp)
+   apply(intro get_rule; intro allI)
+   apply (intro seq_rule[of _ _ "(\<lambda>_ y. high y - i y < high e - i e)"])
+    apply (simp add: spec_def put_def put_state_def swap_def get_state_def i_Env_def)
+    apply (linarith)
+   apply(intro allI; simp)
+   apply(intro get_rule; intro allI)
+   apply(simp add: spec_def put_def get_state_def put_state_def low_Env_def)
+   apply (intro seq_rule[of _ _ "(\<lambda>x y. i e = i y)"])
+   apply (simp add: spec_def put_def put_state_def swap_def get_state_def xs_Env_def i_Env_def)
+   apply(intro allI; simp)
+   apply(intro get_rule; intro allI)
+   apply (intro seq_rule[of _ _ "(\<lambda>x y. i e < i y)"])
+   apply (simp add: spec_def put_def put_state_def swap_def get_state_def i_Env_def)
+   apply(intro allI; simp)
+   apply(intro get_rule; intro allI)
+  by(simp add: spec_def put_def get_state_def put_state_def low_Env_def)
 
 subsubsection\<open>Invariants\<close>
 lemma inc_lowbound_invariantRed: "spec inc_lowbound_inv1 inc_lowbound (GG low_invariant_is_0_Env)"
+  unfolding inc_lowbound_inv1_def loop_update_action_pre_def  GG_def low_invariant_is_0_Env_def
   apply(simp_all add: inc_lowbound_def)
-  apply (simp_all add: inc_lowbound_inv1_def loop_update_action_pre_def low_invariant_is_0_Env_def spec_def  get_def get_state_def return_def put_def put_state_def GG_def)
-  apply(simp add: low_Env_def i_Env_def xs_Env_def swap_def)
-  using less_Suc_eq by auto
+  apply(intro get_rule; intro allI; simp)
+  apply(intro seq_rule[of _ _ "(\<lambda>x e. xs e ! low e = 0 \<and>  (\<forall>x<low e. xs e ! x = 0))"])
+   apply (simp add: spec_def put_def put_state_def swap_def get_state_def xs_Env_def)
+  apply(intro allI; simp)
+  apply(intro get_rule; intro allI)
+  apply(intro seq_rule[of _ _ "(\<lambda>x e. xs e ! low e = 0 \<and> (\<forall>x<low e. xs e ! x = 0))"])
+   apply (simp add: spec_def put_def put_state_def get_state_def i_Env_def)
+  apply(intro allI; simp)
+  apply(intro get_rule; intro allI)
+   apply (simp add: spec_def put_def put_state_def get_state_def low_Env_def)
+  using less_antisym by blast
+
 
 lemma inc_lowbound_invariantWhite: "spec inc_lowbound_inv2  inc_lowbound (GG invariant_low_to_j_is_1_Env)"
+  unfolding inc_lowbound_inv2_def loop_update_action_pre_def  GG_def invariant_low_to_j_is_1_Env_def
   apply(simp_all add: inc_lowbound_def)
-  apply (simp_all add: inc_lowbound_inv2_def loop_update_action_pre_def invariant_low_to_j_is_1_Env_def spec_def  get_def get_state_def return_def put_def put_state_def GG_def)
-  apply(simp add: low_Env_def i_Env_def xs_Env_def swap_def)
-  using less_Suc_eq by auto
+  apply(intro get_rule; intro allI; simp)
+  apply(intro seq_rule[of _ _ "(\<lambda>x e. xs e ! low e = 0 \<and> (\<forall>x. low e \<le> x \<and> x < i e \<longrightarrow> xs e ! x = Suc 0))"])
+   apply (simp add: spec_def put_def put_state_def swap_def get_state_def xs_Env_def)
+   apply(intro allI)
+  apply(intro get_rule; intro allI)
+  apply(intro seq_rule[of _ _ "(\<lambda>x e. xs e ! low e = 0 \<and> (\<forall>x<low e. xs e ! x = 0))"])
+   apply (simp add: spec_def put_def put_state_def get_state_def i_Env_def)
+  apply(intro allI; simp)
+  apply(intro get_rule; intro allI)
+   apply (simp add: spec_def put_def put_state_def get_state_def low_Env_def)
+  sorry
 
 lemma inc_lowbound_invariantBlue: "spec inc_lowbound_inv3  inc_lowbound (GG high_invariant_is_2_Env)"
+  unfolding inc_lowbound_inv3_def loop_update_action_pre_def  GG_def high_invariant_is_2_Env_def
   apply(simp_all add: inc_lowbound_def)
-  apply (simp_all add: inc_lowbound_inv3_def loop_update_action_pre_def high_invariant_is_2_Env_def spec_def  get_def get_state_def return_def put_def put_state_def GG_def)
-  by(simp add: low_Env_def i_Env_def xs_Env_def swap_def)
+  apply(intro get_rule; intro allI; simp)
+  apply(intro seq_rule[of _ _ "(\<lambda>x e. \<forall>x \<ge> high e. xs e ! x = 2)"])
+   apply (simp add: spec_def put_def put_state_def swap_def get_state_def xs_Env_def)
+  apply(intro allI; simp)
+  apply(intro get_rule; intro allI)
+  apply(intro seq_rule[of _ _ "(\<lambda>x e. \<forall>x \<ge> high e. xs e ! x = 2)"])
+   apply (simp add: spec_def put_def put_state_def get_state_def i_Env_def)
+  apply(intro allI; simp)
+  apply(intro get_rule; intro allI)
+  by (simp add: spec_def put_def put_state_def get_state_def low_Env_def)
 
 definition inc_lowbound_inv :: "env \<Rightarrow> bool" where
 "inc_lowbound_inv s \<equiv> (inc_lowbound_inv3 s \<and> inc_lowbound_inv2 s \<and> inc_lowbound_inv1 s)"
 
 lemma inc_lowbound_invariants: "spec inc_lowbound_inv  inc_lowbound (GG invariants_Env)"
-  by (metis (mono_tags, lifting) GG_def inc_lowbound_inv_def inc_lowbound_invariantBlue inc_lowbound_invariantRed inc_lowbound_invariantWhite invariants_Env_def spec_def split_def)
+  unfolding  inc_lowbound_inv_def inc_lowbound_inv1_def inc_lowbound_inv2_def inc_lowbound_inv3_def loop_update_action_pre_def invariants_Env_def  GG_def high_invariant_is_2_Env_def low_invariant_is_0_Env_def invariant_low_to_j_is_1_Env_def 
+  apply(simp_all add: inc_lowbound_def)
+  apply(intro get_rule; intro allI; simp)
+  apply(intro seq_rule[of _ _ "(\<lambda>x e. xs e ! low e = 0 \<and> (\<forall>x\<ge>high e. xs e ! x = 2) \<and> (\<forall>x<low e. xs e ! x = 0))"])
+  apply (simp add: spec_def put_def put_state_def get_def swap_def get_state_def xs_Env_def)
+  apply(intro allI; simp)
+  apply(intro get_rule; intro allI)
+  apply(intro seq_rule[of _ _ "(\<lambda>x e. xs e ! i e = 1 \<and> xs e ! low e = 0 \<and> (\<forall>x<low e. xs e ! x = 0) \<and> (\<forall>x. low e \<le> x \<and> x < i e \<longrightarrow> xs e ! x = 1))"])
+  apply (simp add: spec_def put_def put_state_def get_def swap_def get_state_def xs_Env_def i_Env_def low_Env_def)
+  apply(intro allI; simp)
+  apply(intro get_rule; intro allI)
+  apply (simp add: spec_def put_def put_state_def get_def swap_def get_state_def low_Env_def)
+  apply(intro allI)
+
+ (* by (metis  inc_lowbound_invariantBlue inc_lowbound_invariantRed inc_lowbound_invariantWhite invariants_Env_def spec_def split_def)*)
 
 subsection\<open>Dec_highbound Invariants\<close>
-
+                                            
 lemma dec_highbound_spec: "spec (dec_highbound_pre e) dec_highbound (GG (dec_highbound_post e))"
+  unfolding dec_highbound_pre_def loop_update_action_pre_def GG_def dec_highbound_post_def loop_update_action_post_def
+  apply(simp_all add: dec_highbound_def)
+  apply(intro get_rule; intro allI; simp)
+  apply(intro conj_rule_right)
+   apply(intro seq_rule[of _ _ "(\<lambda>_ y. high y < length (xs e))"])
+        apply (simp add: spec_def put_def put_state_def get_state_def high_Env_def)
+           apply(linarith)
+           apply(intro allI; simp)
+           apply(intro get_rule; intro allI; simp)
+           apply (simp add: spec_def put_def put_state_def get_state_def xs_Env_def)
+           apply(intro seq_rule[of _ _ "(\<lambda>_ y. (xs e)!(i e) = 2\<and> (high e = high y + 1))"])
+           apply (simp add: spec_def put_def put_state_def get_state_def high_Env_def)
+           apply(intro allI; simp)
+           apply(intro get_rule; intro allI; simp)
+           apply (simp add: spec_def put_def put_state_def get_state_def xs_Env_def)
+          apply(intro seq_rule[of _ _ "(\<lambda>_ y.(xs e)!(i e) = 2 \<and> low e = low y)"])
+           apply (simp add: spec_def put_def put_state_def get_state_def high_Env_def)
+           apply(intro allI; simp)
+          apply(intro get_rule; intro allI; simp)
+             apply (simp add: spec_def put_def put_state_def get_state_def xs_Env_def)
+        apply(intro seq_rule[of _ _ "(\<lambda>_ y. (xs e)!(i e) = 2 \<and> i e = i y \<and> xs e = xs y)"])
+             apply (simp add: spec_def put_def put_state_def get_state_def high_Env_def)
+           apply(intro allI; simp)
+         apply(intro get_rule; intro allI; simp)
+        apply (simp add: spec_def put_def put_state_def get_state_def xs_Env_def)
+        apply(intro seq_rule[of _ _ "(\<lambda>_ y. (xs y)!(high y) = 2 \<and> (high e = high y + 1) \<and> xs e = xs y)"])
+        apply (simp add: spec_def put_def put_state_def get_state_def high_Env_def)
+           apply(intro allI; simp)
+       apply(intro get_rule; intro allI; simp)
+       apply (simp add: spec_def put_def put_state_def get_state_def xs_Env_def swap_def)
+       apply(intro allI)
+  sledgehammer
+
+
+           apply(intro get_rule; intro allI; simp)
+       apply (simp add: spec_def put_def put_state_def get_state_def xs_Env_def)
+
+          apply(intro allI)
+  apply(auto)
+sledgehammer
+
+
+           apply(auto)
+
   apply(simp_all add: dec_highbound_def)
   apply (simp_all add: spec_def)
   apply(simp_all add: dec_highbound_pre_def loop_update_action_pre_def add_high_def)
@@ -370,35 +520,34 @@ lemma dec_highbound_invariants: "spec dec_highbound_inv dec_highbound (GG invari
   by (metis (mono_tags, lifting) GG_def dec_highbound_inv_def dec_highbound_invariantBlue dec_highbound_invariantRed dec_highbound_invariantWhite invariants_Env_def spec_def split_def)
 
 subsection\<open>Inc_index Invariants\<close>
-
 lemma inc_index_spec: "spec (inc_index_pre e) inc_index (GG (inc_index_post e))"
+  unfolding inc_index_pre_def loop_update_action_pre_def GG_def inc_index_post_def loop_update_action_post_def
   apply(simp_all add: inc_index_def)
-  apply (intro get_rule)
-  apply (simp_all add: spec_def)
-  apply(simp_all add: inc_index_pre_def loop_update_action_pre_def)
-  apply(simp_all add: get_def get_state_def return_def put_def put_state_def GG_def)
-  apply(simp_all add: inc_index_post_def loop_update_action_post_def i_Env_def)
+  apply(intro get_rule; intro allI;simp)
+  apply(intro conj_rule_right)
+  apply (simp_all add: spec_def put_def put_state_def get_state_def i_Env_def)
   by linarith
 
 subsubsection\<open>Invariants\<close>
 lemma inc_index_invariantRed: "spec inc_index_inv1 inc_index (GG low_invariant_is_0_Env)"
+  unfolding inc_index_inv1_def loop_update_action_pre_def  GG_def low_invariant_is_0_Env_def
   apply(simp_all add: inc_index_def)
-  apply (simp_all add: spec_def inc_index_inv1_def loop_update_action_pre_def low_invariant_is_0_Env_def)
-  apply(simp_all add:  low_invariant_is_0_Env_def get_def get_state_def return_def put_def put_state_def GG_def)
-  by(simp_all add:  i_Env_def)
+  apply(intro get_rule; intro allI; simp)
+  by (simp add: spec_def i_Env_def put_def get_state_def put_state_def)
+
 
 lemma inc_index_invariantWhite: "spec inc_index_inv2 inc_index (GG invariant_low_to_j_is_1_Env)"
-  apply(simp_all add: inc_index_def)         
-  apply (simp_all add: spec_def inc_index_inv2_def loop_update_action_pre_def invariant_low_to_j_is_1_Env_def)
-  apply(simp_all add:  invariant_low_to_j_is_1_Env_def get_def get_state_def return_def put_def put_state_def GG_def)
-  apply(simp_all add:  i_Env_def)
-  using less_SucE by auto
+  unfolding inc_index_inv2_def loop_update_action_pre_def  GG_def invariant_low_to_j_is_1_Env_def
+  apply(simp_all add: inc_index_def)
+  apply(intro get_rule; intro allI; simp)
+  apply (simp add: spec_def i_Env_def put_def get_state_def put_state_def)
+  using less_SucE by blast
 
 lemma inc_index_invariantBlue: "spec inc_index_inv3 inc_index (GG high_invariant_is_2_Env)"
+  unfolding inc_index_inv3_def loop_update_action_pre_def  GG_def high_invariant_is_2_Env_def
   apply(simp_all add: inc_index_def)
-  apply (simp_all add: spec_def inc_index_inv3_def loop_update_action_pre_def high_invariant_is_2_Env_def)
-  apply(simp_all add:  high_invariant_is_2_Env_def get_def get_state_def return_def put_def put_state_def GG_def)
-  by(simp add:  i_Env_def)
+  apply(intro get_rule; intro allI; simp)
+  by (simp add: spec_def i_Env_def put_def get_state_def put_state_def)
 
 definition inc_index_inv :: "env \<Rightarrow> bool" where
 "inc_index_inv s \<equiv> (inc_index_inv3 s \<and> inc_index_inv2 s \<and> inc_index_inv1 s)"
@@ -466,7 +615,7 @@ lemma termination_loop_update_action:
   using loop_update_action_post_def loop_update_action_prepost by blast
 
 subsection\<open>DNFP proof\<close>
-lemma dnfp_prepost: "\<lbrakk>(mk_rec arr l j h) = e; dnfp_pre e; dnfp_pre_aux e; length arr = n; snd(run_state (dnfp_mon n) e) = e2 \<rbrakk> \<Longrightarrow> dnfp_post e e2"
+lemma dnfp_prepost: "spec (dnfp_pre e) (dnfp_mon n) (GG(dnfp_post e))"
   apply(induction n rule:dnfp_mon.induct)
   apply(simp add: mk_rec_def dnfp_pre_def snd_def dnfp_post_def high_invariant_is_2_def loop_update_action_post_def)
    apply force
